linking/linking.v
@@ -369,10 +369,11 @@ Definition main_sig := mksignature nil (Some Tint) cc_default.
 Definition initial_core (tt: ge_ty) (v: val) (args: list val)
   : option (linker N my_cores) :=
   if v is Vptr id ofs then 
+  if Int.eq ofs Int.zero then
   if my_fn_tbl id is Some ix then
   if initCore my_cores main_sig ix (Vptr id Int.zero) args is Some c 
   then Some (mkLinker my_fn_tbl (CallStack.singl c))
-  else None else None else None.
+  else None else None else None else None.
 
 (* Functions suffixed w/ 0 always operate on the running core on the (top *)
 (* of the) call stack.                                                    *)
